add tech/

coq_alt/Ltms/syntax.v
@@ -6,49 +6,16 @@ Require Import CSC.Util.HasEquality CSC.Util.Convenience CSC.Util.NoDupInv.
 
 From RecordUpdate Require Import RecordSet.
 
-(** These are the locs from the L³ paper by Ahmed, Fluet, and Morrisett *)
-Inductive Loc : Type :=
-| LConst : loc -> vart -> Loc
-| LVar : vart -> Loc
-.
-Definition Loc_eqb (l1 l2 : Loc) : bool :=
-  match l1, l2 with
-  | LConst l1 v1, LConst l2 v2 => andb (l1 == l2) (v1 == v2)
-  | LVar v1, LVar v2 => (v1 == v2)
-  | _, _ => false
-  end
-.
-Lemma Loc_eqb_eq l0 l1 :
-  Loc_eqb l0 l1 = true <-> l0 = l1.
-Proof.
-  split; intros H; destruct l0, l1; cbn in *; try easy;
-  try ((change ((l == l0) = true) in H + change ((v == v0) = true) in H);
-       apply eqb_eq in H; subst; easy).
-  eq_to_defeq vareq; eq_to_defeq loc_eqb.
-  inv H; eq_to_defeq loc_eqb. split; eauto. eq_to_defeq vareq.
-  inv H; eq_to_defeq vareq.
-Qed.
-#[export]
-Instance Loceq__Instance : HasEquality Loc := {
-  eq := Loc_eqb ;
-  eqb_eq := Loc_eqb_eq ;
-}.
 (** Values are numbers, pairs, capabilities, and pointers *)
 Inductive value : Type :=
 | Vnat : nat -> value
 | Vpair : value -> value -> value
-| Vcap : value
-| Vptr : loc -> vart -> value
-| Vpack : Loc -> value -> value
 .
 Coercion Vnat : nat >-> value.
 Fixpoint value_eqb (v1 v2 : value) : bool :=
   match v1, v2 with
   | Vnat n1, Vnat n2 => Nat.eqb n1 n2
   | Vpair v0 v1, Vpair v0' v1' => andb (value_eqb v0 v0') (value_eqb v1 v1')
-  | Vcap, Vcap => true
-  | Vptr l0 x0, Vptr l1 x1 => andb (l0 == l1) (x0 == x1)
-  | Vpack l0 v0, Vpack l1 v1 => andb (l0 == l1) (value_eqb v0 v1)
   | _, _ => false
   end
 .
@@ -58,15 +25,10 @@ Proof.
   revert v2; induction v1; cbn; split; intros.
   - destruct v2; try easy. apply Nat.eqb_eq in H; inv H; reflexivity.
   - destruct v2; inv H; apply Nat.eqb_refl.
-  - destruct v2; inv H. eq_to_defeq value_eqb. apply IHv1_1 in H; apply IHv1_2 in H0.
-    subst. reflexivity.
-  - inv H; cbn. eq_to_defeq value_eqb; split. now apply IHv1_1. now apply IHv1_2.
-  - destruct v2; inv H. reflexivity.
-  - destruct v2; inv H. reflexivity.
-  - destruct v2; inv H; eq_to_defeq loc_eqb. eq_to_defeq vareq.
-  - destruct v2; inv H; eq_to_defeq loc_eqb. split; eq_to_defeq vareq.
-  - destruct v2; inv H; eq_to_defeq Loc_eqb. apply IHv1 in H0; subst. reflexivity.
-  - destruct v2; inv H; eq_to_defeq Loc_eqb; split; try easy. now apply IHv1.
+  - inv H; cbn. destruct v2; inv H1. eq_to_defeq value_eqb.
+    eapply IHv1_1 in H. eapply IHv1_2 in H0. now subst.
+  - destruct v2; inv H. eq_to_defeq value_eqb; split. now eapply IHv1_1.
+    now eapply IHv1_2.
 Qed.
 #[export]
 Instance valueeq__Instance : HasEquality value := {
@@ -79,13 +41,11 @@ Inductive expr : Type :=
 | Xval (v : value) : expr
 | Xvar (x : vart) : expr
 | Xbinop (symb : binopsymb) (lhs rhs : expr) : expr
-| Xget (e0 e1 e2 : expr) : expr
-| Xset (e0 e1 e2 e3 : expr) : expr
+| Xget (x : vart) (e0 e1 : expr) : expr
+| Xset (x : vart) (e0 e1 e2 : expr) : expr
 | Xlet (x : vart) (e0 e1 : expr) : expr
-| Xnew (γ : vart) (e__object e__count : expr) : expr (* the γ here is a hack for preservation *)
-| Xdel (e : expr) : expr
-| Xunpack (γ x : vart) (e0 e1 : expr) : expr
-| Xpack (ℓ e : expr) : expr
+| Xnew (x : vart) (e__object e__count e : expr) : expr (* the γ here is a hack for preservation *)
+| Xdel (x : vart) : expr
 | Xpair (e1 e2 : expr) : expr
 | Xunpair (x1 x2 : vart) (e1 e2 : expr) : expr
 | Xreturn (e : expr) : expr
@@ -97,13 +57,10 @@ Inductive expr : Type :=
 Definition exprmap (h : expr -> expr) (e : expr) :=
   match e with
   | Xbinop b lhs rhs => Xbinop b (h lhs) (h rhs)
-  | Xget e0 e1 e2 => Xget (h e0) (h e1) (h e2)
-  | Xset e0 e1 e2 e3 => Xset (h e0) (h e1) (h e2) (h e3)
+  | Xget x e1 e2 => Xget x (h e1) (h e2)
+  | Xset x e1 e2 e3 => Xset x (h e1) (h e2) (h e3)
   | Xlet x e0 e1 => Xlet x (h e0) (h e1)
-  | Xnew γ e1 e2 => Xnew γ (h e1) (h e2)
-  | Xdel e => Xdel (h e)
-  | Xunpack x ℓ e0 e1 => Xunpack x ℓ (h e0) (h e1)
-  | Xpack ℓ e => Xpack ℓ (h e)
+  | Xnew x e1 e2 e3 => Xnew x (h e1) (h e2) (h e3)
   | Xpair e1 e2 => Xpair (h e1) (h e2)
   | Xunpair x1 x2 e1 e2 => Xunpair x1 x2 (h e1) (h e2)
   | Xreturn e => Xreturn (h e)
@@ -117,20 +74,15 @@ Inductive evalctx : Type :=
 | Khole : evalctx
 | KbinopL (b : binopsymb) (K : evalctx) (e : expr) : evalctx
 | KbinopR (b : binopsymb) (v : value) (K : evalctx) : evalctx
-| KgetL (K : evalctx) (e0 e1 : expr) : evalctx
-| KgetM (v : value) (K : evalctx) (e1 : expr) : evalctx
-| KgetR (v0 v1 : value) (K : evalctx) : evalctx
-| KsetL (K : evalctx) (e0 e1 e2 : expr) : evalctx
-| KsetM0 (v : value) (K : evalctx) (e0 e1 : expr) : evalctx
-| KsetM1 (v0 v1 : value) (K : evalctx) (e : expr) : evalctx
-| KsetR (v0 v1 v2 : value) (K : evalctx) : evalctx
+| KgetL (x : vart) (K : evalctx) (e1 : expr) : evalctx
+| KgetR (x : vart) (v0 : value) (K : evalctx) : evalctx
+| KsetL (x : vart) (v : value) (K : evalctx) (e0 e1 : expr) : evalctx
+| KsetM (x : vart) (v0 v1 : value) (K : evalctx) (e : expr) : evalctx
+| KsetR (x : vart) (v0 v1 v2 : value) (K : evalctx) : evalctx
 | Klet (x : vart) (K : evalctx) (e : expr) : evalctx
-| KnewL (γ : vart) (K : evalctx) (e : expr) : evalctx
-| KnewR (γ : vart) (v : value) (K : evalctx) : evalctx
-| Kdel (K : evalctx) : evalctx
-| Kunpack (γ x : vart) (K : evalctx) (e : expr) : evalctx
-| KpackL (K : evalctx) (e : expr) : evalctx
-| KpackR (ℓ : value) (K : evalctx) : evalctx
+| KnewL (x : vart) (K : evalctx) (e0 e1 : expr) : evalctx
+| KnewM (x : vart) (v : value) (K : evalctx) (e : expr) : evalctx
+| KnewR (x : vart) (v0 v1 : value) (K : evalctx) : evalctx
 | KpairL (K : evalctx) (e : expr) : evalctx
 | KpairR (v : value) (K : evalctx) : evalctx
 | Kunpair (x1 x2 : vart) (K : evalctx) (e : expr) : evalctx
@@ -141,20 +93,14 @@ Inductive evalctx : Type :=
 (** Pre-Types of S *)
 Inductive pre_ty : Type :=
 | Tnat : pre_ty
-| Tptr : Loc -> pre_ty
-| Tcap : Loc -> pre_ty -> pre_ty
 | Tpair : pre_ty -> pre_ty -> pre_ty
-| Texists : vart -> pre_ty -> pre_ty
 .
 #[global]
 Notation "'Tℕ'" := (Tnat).
 Fixpoint pre_ty_eqb (t1 t2 : pre_ty) : bool :=
   match t1, t2 with
   | Tnat, Tnat => true
-  | Tptr l1, Tptr l2 => (l1 == l2)
-  | Tcap l1 t1, Tcap l2 t2 => andb (l1 == l2) (pre_ty_eqb t1 t2)
   | Tpair t1 t2, Tpair t1' t2' => andb (pre_ty_eqb t1 t1') (pre_ty_eqb t2 t2')
-  | Texists x t1, Texists y t2 => andb (x == y) (pre_ty_eqb t1 t2)
   | _, _ => false
   end
 .
@@ -163,21 +109,13 @@ Lemma pre_ty_eqb_eq t0 t1 :
 Proof.
   split; revert t1; induction t0; intros.
   - destruct t1; now cbn.
-  - destruct t1; cbn in H; try easy. eq_to_defeq Loc_eqb.
-  - destruct t1; cbn in H; try easy. eq_to_defeq Loc_eqb.
-    specialize (IHt0 t1 H0); subst; reflexivity.
   - destruct t1; cbn in H; try easy. eq_to_defeq pre_ty_eqb.
     specialize (IHt0_1 t1_1 H); specialize (IHt0_2 t1_2 H0); subst.
     reflexivity.
-  - destruct t1; cbn in H; try easy. eq_to_defeq vareq.
-    specialize (IHt0 t1 H0); subst; reflexivity.
   - now destruct t1.
   - destruct t1; try easy; inv H; cbn; eq_to_defeq Loc_eqb.
-  - destruct t1; try easy; inv H; cbn; eq_to_defeq Loc_eqb.
-    split; eq_to_defeq Loc_eqb. eapply IHt0; eauto.
-  - destruct t1; inv H. cbn; eq_to_defeq eq. split; eauto.
-  - destruct t1; try easy; inv H; cbn; eq_to_defeq vareq; split;
-    eq_to_defeq vareq; eapply IHt0; eauto.
+    split; eq_to_defeq Loc_eqb. eapply IHt0_1; eauto.
+    eapply IHt0_2; eauto.
 Qed.
 #[export]
 Instance pre_tyeq__Instance : HasEquality pre_ty := {
